Prove monotonicity fully by well-founded induction. To cleanup!

ecoop17/dsubsup_total_rec_monotone_part2.v
@@ -120,41 +120,146 @@ val_type_func
 
 Argument scopes are [list_scope list_scope _ nat_scope _]
  *)
-Definition val_type_args := fun (env GH : list vl) (T : ty) (n : nat) (v : vl) =>
-  (existT (fun _ : list vl => {_ : list vl & {_ : ty & {_ : nat & vl}}})
-     env
-     (existT (fun _ : list vl => {_ : ty & {_ : nat & vl}}) GH
-        (existT (fun _ : ty => {_ : nat & vl}) T
-           (existT (fun _ : nat => vl) n v)))).
-Check val_type_args.
+(* Definition val_type_args := fun (env GH : list vl) (T : ty) (n : nat) (v : vl) => *)
+(*   (existT (fun _ : list vl => {_ : list vl & {_ : ty & {_ : nat & vl}}}) *)
+(*      env *)
+(*      (existT (fun _ : list vl => {_ : ty & {_ : nat & vl}}) GH *)
+(*         (existT (fun _ : ty => {_ : nat & vl}) T *)
+(*            (existT (fun _ : nat => vl) n v)))). *)
+(* Check val_type_args. *)
 
-Lemma unfold_val_type_less: forall env GH T n v, val_type env GH T n v = val_type_func (val_type_args env GH T n v).
-Proof.
-  intros. unfold val_type. reflexivity.
-Qed.
-(* val_type_args *)
-(*      : list vl -> *)
-(*        list vl -> *)
-(*        ty -> *)
-(*        nat -> *)
-(*        vl -> {_ : list vl & {_ : list vl & {_ : ty & {_ : nat & vl}}}} *)
-Check val_type_func.
-(*
-val_type_func
-     : forall
-         recarg : {_ : list vl & {_ : list vl & {_ : ty & {_ : nat & vl}}}},
-       let env := projT1 recarg in
-       let GH := projT1 (projT2 recarg) in
-       let T := projT1 (projT2 (projT2 recarg)) in
-       let n := projT1 (projT2 (projT2 (projT2 recarg))) in
-       let v := projT2 (projT2 (projT2 (projT2 recarg))) in Prop
- *)
+(* Lemma unfold_val_type_less: forall env GH T n v, val_type env GH T n v = val_type_func (val_type_args env GH T n v). *)
+(* Proof. *)
+(*   intros. unfold val_type. reflexivity. *)
+(* Qed. *)
+(* (* val_type_args *) *)
+(* (*      : list vl -> *) *)
+(* (*        list vl -> *) *)
+(* (*        ty -> *) *)
+(* (*        nat -> *) *)
+(* (*        vl -> {_ : list vl & {_ : list vl & {_ : ty & {_ : nat & vl}}}} *) *)
+(* Check val_type_func. *)
+(* (* *)
+(* val_type_func *)
+(*      : forall *)
+(*          recarg : {_ : list vl & {_ : list vl & {_ : ty & {_ : nat & vl}}}}, *)
+(*        let env := projT1 recarg in *)
+(*        let GH := projT1 (projT2 recarg) in *)
+(*        let T := projT1 (projT2 (projT2 recarg)) in *)
+(*        let n := projT1 (projT2 (projT2 (projT2 recarg))) in *)
+(*        let v := projT2 (projT2 (projT2 (projT2 recarg))) in Prop *)
+(*  *) *)
+(* Print val_type_func. *)
+
+Print termRel.
+Definition natPair := {_ : nat & nat}.
+(* Definition argPair : Set := ((ty * nat)). *)
+Definition argPair := (ty * nat)%type.
+Program Definition natPairI : nat -> nat -> natPair :=
+  fun n1 n2 => existT _ n1 n2.
+Check termRel: natPair -> natPair -> Prop.
 Print val_type_func.
 
-(* Ltac foo := match goal with | H : forall x, ?P x |- _ => idtac P end. *)
-Program Lemma val_type_mon: forall G H T n v, vtp G H T n v -> forall m, m < n -> vtp G H T m v.
+Definition argMeasure T (n: nat): natPair := val_type_measure T n. 
+Check argMeasure.
+Definition argMeasure' (p: argPair) := let '(T, n) := p in argMeasure T n.
+(*(fun T n => val_type_measure T n) *)
+Check (MR termRel ).
+Check (MR termRel argMeasure').
+Definition val_type_termRel := MR termRel argMeasure'.
+(* (fun `(T, n) => argMeasure T n)). *)
+Lemma wf_val_type_termRel : well_founded val_type_termRel.
 Proof.
+  (* unfold val_type_termRel. *)
+  apply measure_wf. apply wf_termRel.
+Qed.
+Hint Resolve wf_val_type_termRel.
+
+Print well_founded.
+
+(* XXX expand p2 to make this hypothesis more usable! *)
+
+Lemma ind_args : forall (P: argPair -> Prop),
+  (forall p1 : argPair,
+      (forall p2 : argPair, val_type_termRel p2 p1 -> P p2) -> P p1) ->
+  forall (p: argPair), P p.
+Proof.
+  intros;
+  eapply well_founded_ind; eauto.
+Qed.
+ 
+Lemma ind_args' : forall (P: ty -> nat -> Prop),
+    (forall T n,
+        (forall T' n', val_type_termRel (T', n') (T, n) -> P T' n') -> P T n) ->
+    forall T n, P T n.
+Proof.
+  (* intros * Hind *. *)
+  (* eapply well_founded_ind; eauto. *)
+  (* intros * Hless. *)
+  (* apply Hind. *)
+  intros * Hind *.
+  pose (p := (T, n)).
+  replace T with (fst p) by reflexivity.
+  replace n with (snd p) by reflexivity.
+  generalize dependent p.
+  clear T n.
+  apply ind_args.
+  intros * Hless.
+  destruct p1 as [T n]; simpl in *.
+  apply Hind.
+  intros *.
+  apply Hless.
+  (* destruct p1 as [T n]; simpl in *. *)
+  (* eapply well_founded_ind; eauto. *)
+  (* intros * Hless. *)
+  (* apply Hind. *)
+Qed.
+
+(* Ltac foo := match goal with | H : forall x, ?P x |- _ => idtac P end. *)
+Program Lemma val_type_mon: forall T n, forall G H v, vtp G H T n v -> forall m, m < n -> vtp G H T m v.
+Proof.
+  intros *.
+  revert G H v.
+  apply ind_args' with (T := T) (n := n).
+  clear T n.
+  intros * Hind * Hvtpn1 * Hmn.
+
+  (* pose (p := (T, n)). *)
+  (* replace T with (fst p) by reflexivity. *)
+  (* replace n with (snd p) by reflexivity. *)
+  (* generalize dependent p. *)
+  (* clear T n. *)
+  (* intro. *)
+  (* apply ind_args with (p := p). *)
+  (* clear p. *)
+  (* intros. *)
+  (* destruct p1 as [T n]; simpl in *. *)
+  (* Until now, this is just setup for well-founded induction. *)
+  
+  destruct T;
+  intros;
+    rewrite val_type_unfold in *;
+      destruct v; ev; repeat split_conj; match_case_analysis.
+  (* We could finish the proof by *)
+  (* all: intros; try assert (Hjn: j < n) by omega; eauto 2. *)
+  (* But let's look how our cases (24 right now!) are solved. *)
+  (* Most cases (12) follow trivially, or by using the induction hypothesis. *)
+
+  (* (* We could finish the proof by *) *)
+  (* (* all: intros; try assert (Hjn: j < n) by omega; eauto 2. *) *)
+  (* But let's look how our cases (24 right now!) are solved. *)
+  (* Most cases (12) follow trivially, or by using the induction hypothesis. *)
+  all: trivial.
+  (* (* A couple (4) follow just by using induction. *) *)
+  (* all: eauto 2. *)
+  (* The other cases (8) have hypothesis for all j < n and have a conclusion for
+     all j < m (with m < n). So we assert that j < n, and then Coq can finish
+     the proof automatically. *)
+  all: intros; try assert (Hjn: j < n) by omega; eauto 2.
+  (* (* A couple (4) follow just by using induction. *) *)
+  all: apply Hind with (n' := n); try smaller_types; assumption.
   (* The proof is by induction on type T, because monotonicity on intersection types follows by induction. *)
+
   (* We proceed by case analysis on values. *)
   (* rewrite vtp_unfold'. *)
 
@@ -193,24 +298,24 @@ Proof.
   (* intros. *)
   (* dependent inversion H0.  ev. *)
   
-  induction T;
-  intros;
-    rewrite val_type_unfold in *;
-      destruct v; ev; repeat split_conj; match_case_analysis.
-  (* We could finish the proof by *)
+  (* induction T; *)
+  (* intros; *)
+  (*   rewrite val_type_unfold in *; *)
+  (*     destruct v; ev; repeat split_conj; match_case_analysis. *)
+  (* (* We could finish the proof by *) *)
+  (* (* all: intros; try assert (Hjn: j < n) by omega; eauto 2. *) *)
+  (* (* But let's look how our cases (24 right now!) are solved. *) *)
+  (* (* Most cases (12) follow trivially, or by using the induction hypothesis. *) *)
+  (* all: trivial. *)
+  (* (* A couple (4) follow just by using induction. *) *)
+  (* all: eauto 2. *)
+  (* (* The other cases (8) have hypothesis for all j < n and have a conclusion for *)
+  (*    all j < m (with m < n). So we assert that j < n, and then Coq can finish *)
+  (*    the proof automatically. *) *)
   (* all: intros; try assert (Hjn: j < n) by omega; eauto 2. *)
-  (* But let's look how our cases (24 right now!) are solved. *)
-  (* Most cases (12) follow trivially, or by using the induction hypothesis. *)
-  all: trivial.
-  (* A couple (4) follow just by using induction. *)
-  all: eauto 2.
-  (* The other cases (8) have hypothesis for all j < n and have a conclusion for
-     all j < m (with m < n). So we assert that j < n, and then Coq can finish
-     the proof automatically. *)
-  all: intros; try assert (Hjn: j < n) by omega; eauto 2.
 
-(* Qed. *)
-Admitted.
+Qed.
+
 
 (* (* This lemma  establishes that val_type indeed defines a value set (vseta). *)
 (*    We need this result in the t_typ/TMem case in the main proof, *)
